atomics/SC_atomics.h
@@ -1,0 +1,19 @@
+#include <stdlib.h>
+#include "threads.h"
+
+// define some special cases of the C11 atomics, since it's hard to specify them in general
+
+typedef struct atom_int atom_int;
+
+// names can't conflict with names of builtins
+atom_int *make_atomic(int v);
+int atom_load(atom_int *tgt);
+void atom_store(atom_int *tgt, int v);
+int atom_CAS(atom_int *tgt, int *c, int v); // returns a bool
+int atom_exchange(atom_int *tgt, int v);
+
+/*atom_ptr make_atom_ptr(void *v);
+void* atomic_load_ptr(atom_ptr *tgt);
+void atomic_store_ptr(atom_ptr *tgt, void *v);
+int atomic_CAS_ptr(atom_ptr *tgt, void **c, void *v); // returns a bool
+void* atomic_exchange_ptr(atom_ptr *tgt, void *v);*/
