atomics/SC_atomics.v
@@ -13,21 +13,183 @@ Set Bullet Behavior "Strict Subproofs".
 (* Warning: it is UNSOUND to use both this file and acq_rel_atomics.v in the same proof! There is
    not yet an operational model that can validate the use of both SC and RA atomics. *)
 
+(* At present, due to complexities in the specifications of the C11 atomics (generics, _Atomic types, etc.), these are specs for wrapper functions for common cases. *)
+
 Section SC_atomics.
 
 Context {CS : compspecs}.
+(*Definition atom_int := Tint I32 Signed {| attr_volatile := false; attr_alignas := Some 32%N |}.*)
+(* Is this what _Atomic int actually should parse to? ask Xavier?
+    In fact, it is almost certainly wrong, and implementation-dependent. *)
+
+Variable atomic_int : type.
+(* Variable is_atomic_version : type -> type -> Prop.
+   Variable _Atomic : type -> type. *)
+Variable atomic_int_at : share -> val -> val -> mpred.
+(*Variable atom_ptr_at : share -> val -> val -> mpred.*)
+
+Definition make_atomic_spec :=
+  WITH v : val
+  PRE [ 1%positive OF tint ]
+    PROP ()
+    LOCAL (temp 1%positive v)
+    SEP ()
+  POST [ tptr atomic_int ]
+   EX p : val,
+    PROP ()
+    LOCAL (temp ret_temp p)
+    SEP (atomic_int_at Ews v p).
 
 Definition AL_type := ProdType (ProdType (ProdType (ProdType (ConstType val)
   (ConstType coPset)) (ConstType coPset))
+  (ArrowType (ConstType val) Mpred)) (ConstType invG).
+
+Program Definition atomic_load_spec := TYPE AL_type
+  WITH p : val, Eo : coPset, Ei : coPset, Q : val -> mpred, inv_names : invG
+  PRE [ 1%positive OF tptr atomic_int ]
+   PROP (subseteq Ei Eo)
+   LOCAL (temp 1%positive p)
+   SEP (|={Eo,Ei}=> EX sh : share, EX v : val, !!(readable_share sh) &&
+              atomic_int_at sh v p * (atomic_int_at sh v p -* |={Ei,Eo}=> Q v))%I
+  POST [ tint ]
+   EX v : val,
+   PROP ()
+   LOCAL (temp ret_temp v)
+   SEP (Q v).
+Next Obligation.
+Proof.
+  repeat intro.
+  unfold PROPx, LOCALx, SEPx; simpl; rewrite !approx_andp; f_equal;
+    f_equal; rewrite -> !sepcon_emp, ?approx_sepcon, ?approx_idem.
+  setoid_rewrite fupd_nonexpansive; do 2 f_equal.
+  rewrite !approx_exp; apply f_equal; extensionality sh.
+  rewrite !approx_exp; apply f_equal; extensionality v. 
+  rewrite !approx_sepcon; f_equal.
+  setoid_rewrite fview_shift_nonexpansive; rewrite approx_idem; auto.
+Qed.
+Next Obligation.
+Proof.
+  repeat intro.
+  rewrite !approx_exp; apply f_equal; extensionality v.
+  unfold PROPx, LOCALx, SEPx; simpl; rewrite !approx_andp; do 2 apply f_equal;
+    rewrite -> !sepcon_emp, ?approx_sepcon, ?approx_idem; auto.
+Qed.
+
+Definition AS_type := ProdType (ProdType (ProdType (ProdType (ConstType (val * val))
+  (ConstType coPset)) (ConstType coPset)) Mpred) (ConstType invG).
+
+Program Definition atomic_store_spec := TYPE AS_type
+  WITH p : val, v : val, Eo : coPset, Ei : coPset, Q : mpred, inv_names : invG
+  PRE [ 1%positive OF tptr atomic_int, 2%positive OF tint ]
+   PROP (subseteq Ei Eo)
+   LOCAL (temp 1%positive p; temp 2%positive v)
+   SEP (|={Eo,Ei}=> EX sh : share, !!(writable_share sh) && atomic_int_at sh Vundef p *
+      (atomic_int_at sh v p -* |={Ei,Eo}=> Q))%I
+  POST [ tvoid ]
+   PROP ()
+   LOCAL ()
+   SEP (Q).
+Next Obligation.
+Proof.
+  repeat intro.
+  unfold PROPx, LOCALx, SEPx; simpl; rewrite !approx_andp; f_equal;
+    f_equal; rewrite -> !sepcon_emp, ?approx_sepcon, ?approx_idem.
+  setoid_rewrite fupd_nonexpansive; do 2 f_equal.
+  rewrite !approx_exp; apply f_equal; extensionality sh.
+  rewrite !approx_sepcon; f_equal.
+  setoid_rewrite fview_shift_nonexpansive; rewrite approx_idem; auto.
+Qed.
+Next Obligation.
+Proof.
+  repeat intro.
+  unfold PROPx, LOCALx, SEPx; simpl; rewrite !approx_andp; do 2 apply f_equal;
+    rewrite -> !sepcon_emp, ?approx_sepcon, ?approx_idem; auto.
+Qed.
+
+Definition ACAS_type := ProdType (ProdType (ProdType (ProdType (ConstType (val * share * val * val * val))
+  (ConstType coPset)) (ConstType coPset))
+  (ArrowType (ConstType val) Mpred)) (ConstType invG).
+
+Program Definition atomic_CAS_spec := TYPE ACAS_type
+  WITH p : val, shc : share, pc : val, c : val, v : val, Eo : coPset, Ei : coPset, Q : val -> mpred, inv_names : invG
+  PRE [ 1%positive OF tptr atomic_int, 2%positive OF tptr tint, 3%positive OF tint ]
+   PROP (readable_share shc; subseteq Ei Eo)
+   LOCAL (temp 1%positive p; temp 2%positive pc; temp 3%positive v)
+   SEP (data_at shc tint c pc; |={Eo,Ei}=> EX sh : share, EX v0 : val,
+      !!(writable_share sh) && atomic_int_at sh v0 p *
+           (atomic_int_at sh (if eq_dec v0 c then v else v0) p -* |={Ei,Eo}=> Q v0))%I
+  POST [ tint ]
+   EX v' : val,
+   PROP ()
+   LOCAL (temp ret_temp (vint (if eq_dec v' c then 1 else 0)))
+   SEP (data_at shc tint c pc; Q v').
+Next Obligation.
+Proof.
+  repeat intro.
+  unfold PROPx, LOCALx, SEPx; simpl; rewrite !approx_andp; f_equal;
+    f_equal; rewrite -> !sepcon_emp, ?approx_sepcon, ?approx_idem.
+  setoid_rewrite fupd_nonexpansive; do 3 f_equal.
+  rewrite !approx_exp; apply f_equal; extensionality sh.
+  rewrite !approx_exp; apply f_equal; extensionality v2.
+  rewrite !approx_sepcon; f_equal.
+  setoid_rewrite fview_shift_nonexpansive; rewrite approx_idem; auto.
+Qed.
+Next Obligation.
+Proof.
+  repeat intro.
+  rewrite !approx_exp; apply f_equal; extensionality vr.
+  unfold PROPx, LOCALx, SEPx; simpl; rewrite !approx_andp; do 2 apply f_equal;
+    rewrite -> !sepcon_emp, ?approx_sepcon, ?approx_idem; auto.
+Qed.
+
+Definition AEX_type := ProdType (ProdType (ProdType (ProdType (ConstType (val * val))
+  (ConstType coPset)) (ConstType coPset))
+  (ArrowType (ConstType val) Mpred)) (ConstType invG).
+
+Program Definition atomic_exchange_spec := TYPE AEX_type
+  WITH p : val, v : val, Eo : coPset, Ei : coPset, Q : val -> mpred, inv_names : invG
+  PRE [ 1%positive OF tptr tint, 2%positive OF tint ]
+   PROP (subseteq Ei Eo)
+   LOCAL (temp 1%positive p; temp 2%positive v)
+   SEP (|={Eo,Ei}=> EX sh : share, EX v0 : val, !!(writable_share sh) &&
+              data_at sh tint v0 p *
+        (data_at sh tint v p -* |={Ei,Eo}=> Q v0))%I
+  POST [ tint ]
+   EX v' : val,
+   PROP ()
+   LOCAL (temp ret_temp v')
+   SEP (Q v').
+Next Obligation.
+Proof.
+  repeat intro.
+  unfold PROPx, LOCALx, SEPx; simpl; rewrite !approx_andp; f_equal;
+    f_equal; rewrite -> !sepcon_emp, ?approx_sepcon, ?approx_idem.
+  setoid_rewrite fupd_nonexpansive; do 2 f_equal.
+  rewrite !approx_exp; apply f_equal; extensionality sh.
+  rewrite !approx_exp; apply f_equal; extensionality v0.
+  rewrite !approx_sepcon; f_equal.
+  setoid_rewrite fview_shift_nonexpansive; rewrite approx_idem; auto.
+Qed.
+Next Obligation.
+Proof.
+  repeat intro.
+  rewrite !approx_exp; apply f_equal; extensionality vr.
+  unfold PROPx, LOCALx, SEPx; simpl; rewrite !approx_andp; do 2 apply f_equal;
+    rewrite -> !sepcon_emp, ?approx_sepcon, ?approx_idem; auto.
+Qed.
+
+(* subspecs for integer operations *)
+Definition ALI_type := ProdType (ProdType (ProdType (ProdType (ConstType val)
+  (ConstType coPset)) (ConstType coPset))
   (ArrowType (ConstType Z) Mpred)) (ConstType invG).
 
-Program Definition load_SC_spec := TYPE AL_type
+Program Definition atomic_load_int_spec := TYPE ALI_type
   WITH p : val, Eo : coPset, Ei : coPset, Q : Z -> mpred, inv_names : invG
-  PRE [ 1%positive OF tptr tint ]
+  PRE [ 1%positive OF tptr atomic_int ]
    PROP (subseteq Ei Eo)
    LOCAL (temp 1%positive p)
    SEP (|={Eo,Ei}=> EX sh : share, EX v : Z, !!(readable_share sh /\ repable_signed v) &&
-              data_at sh tint (vint v) p * (data_at sh tint (vint v) p -* |={Ei,Eo}=> Q v))%I
+              atomic_int_at sh (vint v) p * (atomic_int_at sh (vint v) p -* |={Ei,Eo}=> Q v))%I
   POST [ tint ]
    EX v : Z,
    PROP (repable_signed v)
@@ -52,16 +214,46 @@ Proof.
     rewrite -> !sepcon_emp, ?approx_sepcon, ?approx_idem; auto.
 Qed.
 
-Definition AS_type := ProdType (ProdType (ProdType (ProdType (ConstType (val * Z))
+Lemma atomic_load_int : funspec_sub atomic_load_spec atomic_load_int_spec.
+Proof.
+  apply subsume_subsume.
+  split; auto; split; auto; intros; simpl in *.
+  destruct x2 as ((((p, Eo), Ei), Q), inv_names).
+  intros; match goal with |- ?P |-- |==> ?Q => change (P |-- |==> Q)%I end.
+  intros; iIntros "[_ H] !>".
+  iExists nil, (p, Eo, Ei, fun v => match v with Vint i => Q (Int.signed i) | _ => FF end, inv_names), emp.
+  rewrite emp_sepcon; iSplit.
+  - unfold PROPx, LOCALx, SEPx; simpl.
+    iDestruct "H" as "($ & $ & H & _)"; rewrite sepcon_emp.
+    iMod "H"; iModIntro.
+    iDestruct "H" as (sh v) "[[% H1] H2]".
+    destruct H.
+    iExists sh, (vint v); iFrame.
+    rewrite Int.signed_repr; auto.
+  - iPureIntro.
+    intros; match goal with |- ?P |-- |==> ?Q => change (P |-- |==> Q)%I end.
+    iIntros "(_ & _ & H) !>".
+    unfold PROPx, LOCALx, SEPx; simpl.
+    iDestruct "H" as (r) "(_ & % & Q & _)".
+    destruct H, r; try done.
+    iExists (Int.signed i); iSplit; auto.
+    { iPureIntro; split; auto.
+      apply Int.signed_range. }
+    iSplit; [iSplit; auto|].
+    { rewrite Int.repr_signed; auto. }
+    rewrite sepcon_emp; auto.
+Qed.
+
+Definition ASI_type := ProdType (ProdType (ProdType (ProdType (ConstType (val * Z))
   (ConstType coPset)) (ConstType coPset)) Mpred) (ConstType invG).
 
-Program Definition store_SC_spec := TYPE AS_type
+Program Definition atomic_store_int_spec := TYPE ASI_type
   WITH p : val, v : Z, Eo : coPset, Ei : coPset, Q : mpred, inv_names : invG
-  PRE [ 1%positive OF tptr tint, 2%positive OF tint ]
+  PRE [ 1%positive OF tptr atomic_int, 2%positive OF tint ]
    PROP (repable_signed v; subseteq Ei Eo)
    LOCAL (temp 1%positive p; temp 2%positive (vint v))
-   SEP (|={Eo,Ei}=> EX sh : share, !!(writable_share sh) && data_at_ sh tint p *
-      (data_at sh tint (vint v) p -* |={Ei,Eo}=> Q))%I
+   SEP (|={Eo,Ei}=> EX sh : share, !!(writable_share sh) && atomic_int_at sh Vundef p *
+      (atomic_int_at sh (vint v) p -* |={Ei,Eo}=> Q))%I
   POST [ tvoid ]
    PROP ()
    LOCAL ()
@@ -83,31 +275,48 @@ Proof.
     rewrite -> !sepcon_emp, ?approx_sepcon, ?approx_idem; auto.
 Qed.
 
-Definition ACAS_type := ProdType (ProdType (ProdType (ProdType (ConstType (val * Z * Z))
+Lemma atomic_store_int : funspec_sub atomic_store_spec atomic_store_int_spec.
+Proof.
+  apply subsume_subsume.
+  split; auto; split; auto; intros; simpl in *.
+  destruct x2 as (((((p, v), Eo), Ei), Q), inv_names).
+  intros; match goal with |- ?P |-- |==> ?Q => change (P |-- |==> Q)%I end.
+  intros; iIntros "[_ H] !>".
+  iExists nil, (p, vint v, Eo, Ei, Q, inv_names), emp.
+  rewrite emp_sepcon; iSplit.
+  - unfold PROPx, LOCALx, SEPx; simpl.
+    iDestruct "H" as "(% & $ & H & _)"; rewrite sepcon_emp.
+    destruct H; auto.
+  - iPureIntro.
+    intros; match goal with |- ?P |-- |==> ?Q => change (P |-- |==> Q)%I end.
+    by iIntros "(_ & _ & $)".
+Qed.
+
+Definition ACASI_type := ProdType (ProdType (ProdType (ProdType (ConstType (val * share * val * Z * Z))
   (ConstType coPset)) (ConstType coPset))
   (ArrowType (ConstType Z) Mpred)) (ConstType invG).
 
-Program Definition CAS_SC_spec := TYPE ACAS_type
-  WITH p : val, c : Z, v : Z, Eo : coPset, Ei : coPset, Q : Z -> mpred, inv_names : invG
-  PRE [ 1%positive OF tptr tint, 2%positive OF tint, 3%positive OF tint ]
-   PROP (repable_signed c; repable_signed v; subseteq Ei Eo)
-   LOCAL (temp 1%positive p; temp 2%positive (vint c); temp 3%positive (vint v))
-   SEP (|={Eo,Ei}=> EX sh : share, EX v0 : Z, !!(writable_share sh /\ repable_signed v0) &&
-              data_at sh tint (vint v0) p *
-           (data_at sh tint (vint (if eq_dec v0 c then v else v0)) p -* |={Ei,Eo}=> Q v0))%I
+Program Definition atomic_CAS_int_spec := TYPE ACASI_type
+  WITH p : val, shc : share, pc : val, c : Z, v : Z, Eo : coPset, Ei : coPset, Q : Z -> mpred, inv_names : invG
+  PRE [ 1%positive OF tptr atomic_int, 2%positive OF tptr tint, 3%positive OF tint ]
+   PROP (repable_signed c; repable_signed v; readable_share shc; subseteq Ei Eo)
+   LOCAL (temp 1%positive p; temp 2%positive pc; temp 3%positive (vint v))
+   SEP (data_at shc tint (vint c) pc; |={Eo,Ei}=> EX sh : share, EX v0 : Z,
+      !!(writable_share sh /\ repable_signed v0) && atomic_int_at sh (vint v0) p *
+           (atomic_int_at sh (vint (if eq_dec v0 c then v else v0)) p -* |={Ei,Eo}=> Q v0))%I
   POST [ tint ]
    EX v' : Z,
    PROP (repable_signed v')
    LOCAL (temp ret_temp (vint (if eq_dec v' c then 1 else 0)))
-   SEP (Q v').
+   SEP (data_at shc tint (vint c) pc; Q v').
 Next Obligation.
 Proof.
   repeat intro.
   unfold PROPx, LOCALx, SEPx; simpl; rewrite !approx_andp; f_equal;
     f_equal; rewrite -> !sepcon_emp, ?approx_sepcon, ?approx_idem.
-  setoid_rewrite fupd_nonexpansive; do 2 f_equal.
+  setoid_rewrite fupd_nonexpansive; do 3 f_equal.
   rewrite !approx_exp; apply f_equal; extensionality sh.
-  rewrite !approx_exp; apply f_equal; extensionality v0.
+  rewrite !approx_exp; apply f_equal; extensionality v2.
   rewrite !approx_sepcon; f_equal.
   setoid_rewrite fview_shift_nonexpansive; rewrite approx_idem; auto.
 Qed.
@@ -119,11 +328,52 @@ Proof.
     rewrite -> !sepcon_emp, ?approx_sepcon, ?approx_idem; auto.
 Qed.
 
-Definition AEX_type := ProdType (ProdType (ProdType (ProdType (ConstType (val * Z))
+Lemma atomic_CAS_int : funspec_sub atomic_CAS_spec atomic_CAS_int_spec.
+Proof.
+  apply subsume_subsume.
+  split; auto; split; auto; intros; simpl in *.
+  destruct x2 as ((((((((p, shc), pc), c), v), Eo), Ei), Q), inv_names).
+  intros; match goal with |- ?P |-- |==> ?Q => change (P |-- |==> Q)%I end.
+  intros; iIntros "[_ H] !>".
+  iExists nil, (p, shc, pc, vint c, vint v, Eo, Ei, fun v => match v with Vint i => Q (Int.signed i) | _ => FF end, inv_names), emp.
+  rewrite emp_sepcon; iSplit.
+  - unfold PROPx, LOCALx, SEPx; simpl.
+    iDestruct "H" as "(% & $ & $ & H & _)"; rewrite sepcon_emp.
+    destruct H as (? & ? & ?); iSplit; auto.
+    iMod "H"; iModIntro.
+    iDestruct "H" as (sh v0) "[[% H1] H2]".
+    destruct H2.
+    iExists sh, (vint v0); iFrame.
+    rewrite -> Int.signed_repr by auto.
+    iSplit; first done.
+    if_tac.
+    + subst; rewrite eq_dec_refl; done.
+    + if_tac; last done.
+      match goal with H : vint _ = vint _ |- _ => apply Vint_inj, repr_inj_signed in H end; auto; contradiction.
+  - unfold PROPx, LOCALx, SEPx; simpl.
+    iDestruct "H" as "[% _]".
+    destruct H as [Hc _].
+    iPureIntro.
+    intros; match goal with |- ?P |-- |==> ?Q => change (P |-- |==> Q)%I end.
+    iIntros "(_ & _ & H) !>".
+    iDestruct "H" as (r) "(_ & % & ? & Q & _)".
+    destruct H, r; try done.
+    iExists (Int.signed i); iSplit; auto.
+    { iPureIntro; split; auto.
+      apply Int.signed_range. }
+    iSplit; [iSplit; auto|].
+    { if_tac; if_tac in H; auto; subst.
+      + rewrite Int.repr_signed in H2; contradiction.
+      + apply Vint_inj in H2; subst.
+        rewrite -> Int.signed_repr in H1 by auto; contradiction. }
+    rewrite sepcon_emp; iFrame.
+Qed.
+
+Definition AEXI_type := ProdType (ProdType (ProdType (ProdType (ConstType (val * Z))
   (ConstType coPset)) (ConstType coPset))
   (ArrowType (ConstType Z) Mpred)) (ConstType invG).
 
-Program Definition AEX_SC_spec := TYPE AEX_type
+Program Definition atomic_exchange_int_spec := TYPE AEXI_type
   WITH p : val, v : Z, Eo : coPset, Ei : coPset, Q : Z -> mpred, inv_names : invG
   PRE [ 1%positive OF tptr tint, 2%positive OF tint ]
    PROP (repable_signed v; subseteq Ei Eo)
@@ -153,6 +403,37 @@ Proof.
   rewrite !approx_exp; apply f_equal; extensionality vr.
   unfold PROPx, LOCALx, SEPx; simpl; rewrite !approx_andp; do 2 apply f_equal;
     rewrite -> !sepcon_emp, ?approx_sepcon, ?approx_idem; auto.
+Qed.
+
+Lemma atomic_exchange_int : funspec_sub atomic_exchange_spec atomic_exchange_int_spec.
+Proof.
+  apply subsume_subsume.
+  split; auto; split; auto; intros; simpl in *.
+  destruct x2 as (((((p, v), Eo), Ei), Q), inv_names).
+  intros; match goal with |- ?P |-- |==> ?Q => change (P |-- |==> Q)%I end.
+  intros; iIntros "[_ H] !>".
+  iExists nil, (p, vint v, Eo, Ei, fun v => match v with Vint i => Q (Int.signed i) | _ => FF end, inv_names), emp.
+  rewrite emp_sepcon; iSplit.
+  - unfold PROPx, LOCALx, SEPx; simpl.
+    iDestruct "H" as "(% & $ & H & _)"; rewrite sepcon_emp.
+    destruct H; iSplit; auto.
+    iMod "H"; iModIntro.
+    iDestruct "H" as (sh v0) "[[% H1] H2]".
+    destruct H1.
+    iExists sh, (vint v0); iFrame.
+    rewrite -> Int.signed_repr; auto.
+  - unfold PROPx, LOCALx, SEPx; simpl.
+    iPureIntro.
+    intros; match goal with |- ?P |-- |==> ?Q => change (P |-- |==> Q)%I end.
+    iIntros "(_ & _ & H) !>".
+    iDestruct "H" as (r) "(_ & % & Q & _)".
+    destruct H, r; try done.
+    iExists (Int.signed i); iSplit; auto.
+    { iPureIntro; split; auto.
+      apply Int.signed_range. }
+    iSplit; [iSplit; auto|].
+    { rewrite Int.repr_signed; auto. }
+    rewrite sepcon_emp; iFrame.
 Qed.
 
 End SC_atomics.
